- [Back to Main](../main.md)

# 13. Basics of Proof
### E.g.1) 
- Target
  - The sum of two even integers is even.
- pf.)   
    $`\begin{aligned}
        \textrm{Put } & x=2i, y=2j \textrm{ where } i,j \in \mathbb{Z} \\
        \textrm{Then } & x+y = 2i+2j = 2(i+j)
    \end{aligned}`$

<br>

### E.g.2)
- Target
  - $`A \subseteq B`$
    - where $`A=\{x\in\mathbb{Z}|18 \textrm{ divides } x\}, B = \{x\in\mathbb{Z}|6 \textrm{ divides } x\}`$
- pf.)   
  $`\begin{aligned}
        \textrm{Consider that } & \forall x \in A, \exists y \in \mathbb{Z} \textrm{ s.t. } x = 16y. \\
        \textrm{Then } & x = 16y = 6(3y) \in B. \\
        \textrm{Thus, } & \forall x \in A, x \in B. \\
        \therefore A \subseteq B.
  \end{aligned}`$

<br>

### E.g.)
- Target
  - Prove that $`A\cup(B\cap C) = (A\cup B)\cap(A\cup C)`$
- pf.)   
  - Put $`x \in A\cup(B\cap C)`$.
    - Then, $`(x \in A) \vee (x \in (B\cap C))`$
      - Case 1) $`x\in A`$.
        - Then $`(x \in (A\cup B)) \wedge (x \in (A\cup C))`$.
        - Thus, $`x \in (A\cup B)\cap(A\cup C)`$
      - Case 2) $`x \in (B\cap C)`$
        - Then $`x \in B \Rightarrow x \in (A\cup B)`$.
        - Also, $`x \in C \Rightarrow x \in (A\cup C)`$.
        - Thus, $`x \in (A\cup B)\cap(A\cup C)`$
    - Hence, $`\forall x \in A\cup(B\cap C), x\in (A\cup B)\cap(A\cup C)`$
  - Put $`y \in (A\cup B)\cap(A\cup C)`$
    - Then $`(y \in (A\cup B)) \wedge (y \in (A\cup C)) \Leftrightarrow (y\in A \vee y\in B) \wedge (y\in A \vee y\in C)`$
    - Thus, $`(y \in A) \vee (y\in B \wedge y\in C) \Leftrightarrow y\in A \vee (y\in (B\cap C))`$
    - Hence, $`\forall y \in (A\cup B)\cap(A\cup C), y\in A\cup(B\cap C)`$.
  - $`\therefore A\cup(B\cap C) = (A\cup B)\cap(A\cup C)`$

<br><br>

- [Back to Main](../main.md)